---
cssclasses:
  - center-images
  - center-titles
  - page-black
  - pen-white
date: 2024-09-24
---
2024-11-12

## Ex. 2
$$
x^3+x^2-2x=x(x+2)(x-1)
$$
$$
\begin{align}
\int 2x^2+5x-1 \, dx  & =\frac{A}{x}+\frac{B}{x+2}+\frac{C}{x-1} \\ \\

 & \text{เคลี่ยร์ตัวส่วนเพื่อความสะดวกนการหา A,B,C} \\ \\

2x^2+5x-1 & =A(x+2)(x-1) \\
 & +B(x)(x-1) \\
 & +C(x)(x+2) \\ \\

 & \text{หา A โดยการแทนค่า X = 0} \\ \\

-1 & = A(-2) \to A=\frac{1}{2} \\
-3  & = 6B \to B=-\frac{1}{2} \\
6 & =3C \to C=2 \\

\\
\frac{2x^2+5x-1}{x^3+x^2-2x} & =\frac{1}{2}\cdot \frac{1}{x}- \frac{1}{2} \cdot \frac{1}{x+2}+ \frac{2}{x-1} \\
 & =\frac{1}{2}\int \frac{1}{x}dx- \frac{1}{2}\int \frac{1}{x+2} \, dx +2 \int \frac{1}{x-1} \, dx  \\
 & =\frac{1}{2}\ln|x|-\frac{1}{2}\ln|x+2|+2 \ln|x-1|+C
\end{align}
$$
## 2nd Form

$(ax+b)^n$ 

$$
\begin{align}
\frac{Ax^4+Bx^3+Cx^2+Dx+E}{x^5} & =\frac{A}{x}+\frac{B}{x^2}+\frac{C}{x^3}+\frac{D}{x^4}+\frac{E}{x^5}
\end{align}
$$

### Example 4.

$$
\begin{align}
\frac{2x^2-3x+4}{(x+1)(x-2)^2} & = \frac{A}{x+1}+\frac{B}{x-2}+\frac{C}{(x-2)^2}
\end{align}
$$
$$
\begin{align}
2x^2-3x+4=A(x-2)^2+B(x+1)(x-2)+C(x+1)
\end{align}
$$
$$
\begin{align}
2-3(-1)+4 & =9A \\
9 & =A \\
A & =1 \\
 \\
6 & =3C \\
C & =2 \\
 \\
4 & =A(4)+B(-2)+2 \\
 & =1(4)+B(-2)+2 \\
-2 & =-2B
\end{align}
$$

$$
\begin{align}
\frac{2x^2-3x+4}{(x+1)(x-2)^2} & = \frac{1}{x+1}+\frac{1}{x-2}+\frac{2}{(x-2)^2} \\
\int \frac{2x^2-3x+4}{(x+1)(x-2)^2}  \, dx  & =\int \frac{1}{x+1} \, dx +\int \frac{1}{x-2} \, dx +2\int \frac{1}{(x-2)^2} \,dx \\
 & =\ln|x+1|+\ln |x-2|+2\int \frac{1}{(x-2)^2} \, d(x-2) \\
  & =\ln|x+1|+\ln |x-2|+2\cdot\left( -\frac{1}{x-2} \right)+C \\
\end{align}
$$
### Example 5.

$$
\begin{align}
x-3 & =A(x+1)+B \\
-4 & =B \\
 \\
0-3 & =A(0+1)+B \\
-3 & =A+(-4) \\
A & =1
\end{align}
$$
$$
\begin{align}
\int \frac{2x^2+5x-1}{(x+1)^2} \, dx  & =\int 2+\frac{1}{x+1}-\frac{4}{(x+1)^2} \, dx  \\
 & =2x+\ln|x+1|+\frac{4}{x+1}+C
\end{align}
$$

### Example 6.

$$
\int x+\frac{4}{x^2(x^2+4)} \, dx 
$$
$$
\begin{align}
\frac{x+4}{x^2+(x^2+4)} & =\frac{A}{x}+\frac{B}{x^2}+\frac{Cx+D}{x^2+4} \\
x+4 & =Ax(x^2+4)+B(x^2+4)+(Cx+D)(x^2)
\end{align}
$$
$$
\begin{align}
X & =0 \\
4 & =4B \\
B & =1
\end{align}
$$

แทน x ด้วย 2i โดย i=$\sqrt{ -1 }$

$$
\begin{align}
2i+4 & =A(0)+B(0)+(2Ci+D)(-4) \\
2i+4 & =-8(i-4i)
\end{align}
$$
$$
\begin{align}
C & =-\frac{1}{2} \\
D & =-1
\end{align}
$$
$$
\begin{align}
5 & =5A+5B+(C+D) \\
A & =\frac{1}{4}
\end{align}
$$
$$
\begin{align}
 & = \frac{A}{x}+\frac{B}{x^2}+\frac{Cx+D}{x^2+4} \\
 & = \frac{1}{4} \cdot \frac{1}x+\frac{1}{x^2}-\frac{1}{4} \frac{x}{x^2+4}-\frac{1}{x^2+4} \\
 & =\int \frac{1}{4} \cdot \frac{1}x+\frac{1}{x^2}-\frac{1}{4} \frac{x}{x^2+4}-\frac{1}{x^2+4} \, dx  \\
 & =\frac{1}{4}\ln|x|-\frac{1}{x}-\frac{1}{8}\ln|x^2+4|-\arctan\left( \frac{x}{2} \right)+C
\end{align}
$$
